zoo_parabs/algo: Verify [find].

theories/zoo_parabs/algo.v
@@ -1,13 +1,18 @@
 From zoo Require Import
   prelude.
+From zoo.common Require Import
+  countable.
 From zoo.iris.bi Require Import
   big_op.
+From zoo.iris.base_logic Require Import
+  lib.ghost_var.
 From zoo.language Require Import
   notations.
 From zoo.diaframe Require Import
   diaframe.
 From zoo_std Require Import
   for_
+  mvar
   option.
 From zoo_parabs Require Export
   base
@@ -18,14 +23,20 @@ From zoo_parabs Require Import
 From zoo Require Import
   options.
 
-Implicit Types v pool ctx task : val.
+Implicit Types b : bool.
+Implicit Types v pool ctx task pred found : val.
+Implicit Types o : option val.
 
 Class AlgoG Σ `{pool_G : PoolG Σ} := {
   #[local] algo_G_future_G :: FutureG Σ ;
+  #[local] algo_G_mvar_G :: MvarG Σ ;
+  #[local] algo_G_find_G :: GhostVarG Σ unitO ;
 }.
 
 Definition algo_Σ := #[
-  future_Σ
+  future_Σ ;
+  mvar_Σ ;
+  ghost_var_Σ unitO
 ].
 #[global] Instance subG_algo_Σ Σ `{pool_G : PoolG Σ} :
   subG algo_Σ Σ →
@@ -60,7 +71,7 @@ Section algo_G.
     - iSteps.
   Qed.
 
-  #[local] Lemma algo_for_0_spec Ψ Χ pool ctx scope beg0 beg end_ end0 (chunk : Z) task :
+  #[local] Lemma algo_for_0_spec (Ψ : Z → iProp Σ) (Χ : Z → nat → iProp Σ) pool ctx scope beg0 beg end_ end0 (chunk : Z) task :
     (beg0 ≤ beg ≤ end_ ≤ end0)%Z →
     {{{
       pool_context pool ctx scope ∗
@@ -120,7 +131,7 @@ Section algo_G.
         ( λ _,
           True
         )%I
-      with "[$Hctx HΧ_1]") as (fut1) "(Hctx & #Hfut1_inv & Hfut1_consumer)".
+      with "[$Hctx HΧ_1]") as (fut) "(Hctx & #Hfut_inv & Hfut_consumer)".
       { clear ctx scope. iIntros "%ctx %scope Hctx".
         wp_smart_apply ("HLöb" with "[%] Hctx HΧ_1"); first naive_solver lia.
         { iSteps. }
@@ -129,14 +140,14 @@ Section algo_G.
       wp_smart_apply ("HLöb" with "[%] Hctx HΧ_2") as "(Hctx & HΨ_2)"; first naive_solver lia.
 
       iApply wp_fupd.
-      wp_smart_apply (future_wait_spec with "[$]") as (res) "(H£ & Hctx & Hfut1_result)".
+      wp_smart_apply (future_wait_spec with "[$]") as (res) "(H£ & Hctx & Hfut_result)".
 
-      iMod (future_inv_result_consumer' with "H£ Hfut1_inv Hfut1_result Hfut1_consumer") as "((-> & HΨ_1) & _)".
+      iMod (future_inv_result_consumer' with "H£ Hfut_inv Hfut_result Hfut_consumer") as "((-> & HΨ_1) & _)".
       iDestruct (big_sepL_seqZ_app_2 with "HΨ_1 HΨ_2") as "HΨ"; [naive_solver lia.. |].
       iEval (replace (mid - beg + (end_ - mid))%Z with (end_ - beg)%Z by lia) in "HΨ".
       iSteps.
   Qed.
-  Lemma algo_for_spec Ψ Χ pool sz ctx scope beg end_ chunk task :
+  Lemma algo_for_spec (Ψ : Z → iProp Σ) (Χ : Z → nat → iProp Σ) pool sz ctx scope beg end_ chunk task :
     (beg ≤ end_)%Z →
     {{{
       pool_inv pool sz ∗
@@ -180,7 +191,7 @@ Section algo_G.
     wp_smart_apply (algo_for_0_spec Ψ Χ with "[$]"); first done.
     iSteps.
   Qed.
-  Lemma algo_for_spec_nat Ψ Χ pool sz ctx scope beg end_ chunk task :
+  Lemma algo_for_spec_nat (Ψ : nat → iProp Σ) (Χ : Z → nat → iProp Σ) pool sz ctx scope beg end_ chunk task :
     (0 ≤ beg ≤ end_)%Z →
     {{{
       pool_inv pool sz ∗
@@ -238,7 +249,7 @@ Section algo_G.
     iSteps as "HΨ".
     iApply (big_sepL_seqZ_to_seq' with "HΨ"); lia.
   Qed.
-  Lemma algo_for_spec' Ψ pool sz ctx scope beg end_ chunk task :
+  Lemma algo_for_spec' (Ψ : Z → iProp Σ) pool sz ctx scope beg end_ chunk task :
     (beg ≤ end_)%Z →
     {{{
       pool_inv pool sz ∗
@@ -273,7 +284,7 @@ Section algo_G.
     with "[$Hpool_inv $Hchunk $Hctx] HΦ"); first done.
     { iSteps. }
   Qed.
-  Lemma algo_for_spec_nat' Ψ pool sz ctx scope beg end_ chunk task :
+  Lemma algo_for_spec_nat' (Ψ : nat → iProp Σ) pool sz ctx scope beg end_ chunk task :
     (0 ≤ beg ≤ end_)%Z →
     {{{
       pool_inv pool sz ∗
@@ -316,7 +327,7 @@ Section algo_G.
     iApply (big_sepL_seqZ_to_seq' with "HΨ"); lia.
   Qed.
 
-  Lemma algo_for_each_spec' Ψ pool sz ctx scope beg end_ chunk task :
+  Lemma algo_for_each_spec' (Ψ : Z → iProp Σ) pool sz ctx scope beg end_ chunk task :
     (beg ≤ end_)%Z →
     {{{
       pool_inv pool sz ∗
@@ -397,7 +408,7 @@ Section algo_G.
         rewrite Z.add_simpl_l Nat2Z.id. iSteps.
     }
   Qed.
-  Lemma algo_for_each_spec_nat' Ψ pool sz ctx scope beg end_ chunk task :
+  Lemma algo_for_each_spec_nat' (Ψ : nat → iProp Σ) pool sz ctx scope beg end_ chunk task :
     (0 ≤ beg ≤ end_)%Z →
     {{{
       pool_inv pool sz ∗
@@ -426,8 +437,7 @@ Section algo_G.
     wp_apply (algo_for_each_spec'
       (λ i, Ψ ₊i)
     with "[$Hpool_inv $Hchunk $Hctx Htask]"); first lia.
-    { iDestruct (big_sepL_seq_to_seqZ with "Htask") as "Htask".
-      iEval (rewrite !Z2Nat.id; try lia) in "Htask".
+    { iDestruct (big_sepL_seq_to_seqZ' with "Htask") as "Htask"; [lia.. |].
       iApply (big_sepL_seqZ_impl with "Htask"). iIntros "!> %k % Htask".
       iEval (rewrite Z2Nat.id; try lia) in "Htask".
       iSteps.
@@ -436,7 +446,7 @@ Section algo_G.
     iSteps as "HΨ".
     iApply (big_sepL_seqZ_to_seq' with "HΨ"); lia.
   Qed.
-  Lemma algo_for_each_spec Ψ pool sz ctx scope beg end_ chunk task :
+  Lemma algo_for_each_spec (Ψ : Z → iProp Σ) pool sz ctx scope beg end_ chunk task :
     (beg ≤ end_)%Z →
     {{{
       pool_inv pool sz ∗
@@ -468,7 +478,7 @@ Section algo_G.
       iSteps.
     }
   Qed.
-  Lemma algo_for_each_spec_nat Ψ pool sz ctx scope beg end_ chunk task :
+  Lemma algo_for_each_spec_nat (Ψ : nat → iProp Σ) pool sz ctx scope beg end_ chunk task :
     (0 ≤ beg ≤ end_)%Z →
     {{{
       pool_inv pool sz ∗
@@ -496,6 +506,356 @@ Section algo_G.
     iIntros "% %Φ (Hpool_inv & Hctx & Hchunk & #Htask) HΦ".
 
     wp_apply (algo_for_each_spec_nat' Ψ with "[$Hpool_inv $Hchunk $Hctx] HΦ"); first done.
+    { iApply big_sepL_seq_intro.
+      iSteps.
+    }
+  Qed.
+
+  #[local] Definition find_token γ q :=
+    ghost_var γ (DfracOwn q) ().
+  #[local] Definition find_inv γ (Ψ : Z → iProp Σ) beg end_ v : iProp Σ :=
+    ∃ (i : Z) q,
+    ⌜v = #i⌝ ∗
+    ⌜beg ≤ i < end_⌝%Z ∗
+    find_token γ q ∗
+    Ψ i.
+  #[local] Instance : CustomIpatFormat "find_inv" :=
+    " ( %i &
+        %q &
+        -> &
+        % &
+        Htoken{_{}} &
+        HΨ
+      )
+    ".
+  #[local] Lemma algo_find_seq_spec pool ctx scope beg0 beg end_ end0 pred Ψ (Χ : Z → iProp Σ) found γ q :
+    (beg0 ≤ beg ≤ end_ ≤ end0)%Z →
+    {{{
+      pool_context pool ctx scope ∗
+      mvar_inv found (find_inv γ Ψ beg0 end0) ∗
+      find_token γ q ∗
+      [∗ list] (i : Z) ∈ seqZ beg (end_ - beg),
+        ∀ ctx scope,
+        pool_context pool ctx scope -∗
+        WP pred ctx #i {{ res,
+          ∃ b,
+          ⌜res = #b⌝ ∗
+          pool_context pool ctx scope ∗
+          if b then
+            Ψ i
+          else
+            Χ i
+        }}
+    }}}
+      algo_find_seq ctx #beg #end_ pred found
+    {{{
+      RET ();
+      pool_context pool ctx scope ∗
+      ( mvar_resolved found
+      ∨ find_token γ q ∗
+        [∗ list] i ∈ seqZ beg (end_ - beg),
+          Χ i
+      )
+    }}}.
+  Proof.
+    iIntros "%Hrange %Φ (Hctx & #Hfound_inv & Htoken & Hpred) HΦ".
+
+    iLöb as "HLöb" forall (beg Φ Hrange).
+
+    wp_rec. wp_pures.
+    case_bool_decide; wp_pures.
+
+    - iEval (rewrite seqZ_nil; first lia) in "HΦ".
+      iSteps.
+
+    - wp_apply (mvar_is_unset_spec with "[$]") as ([]) "H"; last iSteps.
+      iClear "H".
+
+      iDestruct (big_sepL_seqZ_cons_1 with "Hpred") as "(H & Hpred)"; first lia.
+      wp_smart_apply (wp_wand with "(H Hctx)") as (res) "(%b & -> & Hctx & H)".
+      destruct b; wp_pures.
+
+      + wp_apply (mvar_set_spec with "[$Hfound_inv $Htoken $H]"); first iSteps.
+        iSteps.
+
+      + wp_apply ("HLöb" with "[%] [$] [$] [Hpred]") as "(Hctx & [#Hfound_resolved | (Htoken & HΧ)])"; first lia.
+        { iEval (replace (beg + 1)%Z with (Z.succ beg) by lia).
+          iEval (replace (end_ - Z.succ beg)%Z with (Z.pred (end_ - beg)) by lia).
+          iFrame.
+        }
+
+        * iSteps.
+
+        * iDestruct (big_sepL_seqZ_cons_2 with "HΧ [H]") as "HΧ"; first lia.
+          { iEval (replace (Z.pred (beg + 1)) with beg by lia).
+            iFrame.
+          }
+          iEval (replace (Z.pred (beg + 1)) with beg by lia) in "HΧ".
+          iEval (replace (Z.succ (end_ - (beg + 1))) with (end_ - beg)%Z by lia) in "HΧ".
+          iSteps.
+  Qed.
+  #[local] Lemma algo_find_0_spec pool ctx scope beg0 beg end_ end0 (chunk : Z) pred Ψ (Χ : Z → iProp Σ) found γ q :
+    (beg0 ≤ beg ≤ end_ ≤ end0)%Z →
+    {{{
+      pool_context pool ctx scope ∗
+      mvar_inv found (find_inv γ Ψ beg0 end0) ∗
+      find_token γ q ∗
+      [∗ list] (i : Z) ∈ seqZ beg (end_ - beg),
+        ∀ ctx scope,
+        pool_context pool ctx scope -∗
+        WP pred ctx #i {{ res,
+          ∃ b,
+          ⌜res = #b⌝ ∗
+          pool_context pool ctx scope ∗
+          if b then
+            Ψ i
+          else
+            Χ i
+        }}
+    }}}
+      algo_find_0 ctx #beg #end_ #chunk pred found
+    {{{
+      RET ();
+      pool_context pool ctx scope ∗
+      ( mvar_resolved found
+      ∨ find_token γ q ∗
+        [∗ list] i ∈ seqZ beg (end_ - beg),
+          Χ i
+      )
+    }}}.
+  Proof.
+    iIntros "%Hrange %Φ (Hctx & #Hfound_inv & Htoken & Hpred) HΦ".
+
+    iLöb as "HLöb" forall (ctx scope beg end_ q Φ Hrange).
+
+    wp_rec. wp_pures.
+    case_bool_decide; wp_pures.
+
+    - iEval (replace (beg + (end_ - beg))%Z with end_ by lia).
+      wp_apply (algo_find_seq_spec with "[$Hctx $Hfound_inv $Htoken $Hpred] HΦ"); first done.
+
+    - wp_apply (mvar_is_unset_spec with "[$]") as ([]) "H"; last iSteps.
+      iClear "H".
+
+      iDestruct "Htoken" as "(Htoken_1 & Htoken_2)".
+
+      pose mid : Z := beg + (end_ - beg) `quot` 2.
+      iEval (replace (end_ - beg)%Z with ((mid - beg) + (end_ - mid))%Z by lia) in "Hpred".
+      iDestruct (big_sepL_seqZ_app with "Hpred") as "(Hpred_1 & Hpred_2)"; [naive_solver lia.. |].
+      iEval (replace (beg + (mid - beg))%Z with mid by lia) in "Hpred_2".
+
+      wp_smart_apply (future_async_spec
+        ( λ res,
+          ⌜res = ()%V⌝ ∗
+          ( mvar_resolved found
+          ∨ find_token γ (q / 2) ∗
+            [∗ list] i ∈ seqZ beg (mid - beg),
+              Χ i
+          )
+        )%I
+        (λ _, True)%I
+        with "[$Hctx Htoken_1 Hpred_1]") as (fut) "(Hctx & #Hfut_inv & Hfut_consumer)".
+      { clear ctx scope. iIntros "%ctx %scope Hctx".
+        wp_smart_apply ("HLöb" with "[%] [$] [$] Hpred_1"); first naive_solver lia.
+        iSteps.
+      }
+
+      wp_smart_apply ("HLöb" with "[%] [$] [$] Hpred_2") as "(Hctx & H)"; first naive_solver lia.
+
+      iApply wp_fupd.
+      wp_smart_apply (future_wait_spec with "[$]") as (res) "(H£ & Hctx & #Hfut_result)".
+
+      iMod (future_inv_result_consumer' with "H£ Hfut_inv Hfut_result Hfut_consumer") as "((-> & [#Hfound_resolved | (Htoken_1 & HΧ_1)]) & _)"; first iSteps.
+      iDestruct "H" as "[#Hfound_resolved | (Htoken_2 & HΧ_2)]"; first iSteps.
+
+      iCombine "Htoken_1 Htoken_2" as "Htoken".
+
+      iDestruct (big_sepL_seqZ_app_2 with "HΧ_1 HΧ_2") as "HΧ"; [naive_solver lia.. |].
+      iEval (replace (mid - beg + (end_ - mid))%Z with (end_ - beg)%Z by lia) in "HΧ".
+
+      iSteps.
+  Qed.
+  Lemma algo_find_spec' (Ψ Χ : Z → iProp Σ) pool sz ctx scope beg end_ chunk pred :
+    (beg ≤ end_)%Z →
+    {{{
+      pool_inv pool sz ∗
+      pool_context pool ctx scope ∗
+      itype_option itype_int chunk ∗
+      [∗ list] (i : Z) ∈ seqZ beg (end_ - beg),
+        ∀ ctx scope,
+        pool_context pool ctx scope -∗
+        WP pred ctx #i {{ res,
+          ∃ b,
+          ⌜res = #b⌝ ∗
+          pool_context pool ctx scope ∗
+          if b then
+            Ψ i
+          else
+            Χ i
+        }}
+    }}}
+      algo_find ctx #beg #end_ chunk pred
+    {{{ (o : option Z),
+      RET ((#@{Z}) <$> o : option val) : val;
+      pool_context pool ctx scope ∗
+      if o is Some i then
+        ⌜beg ≤ i < end_⌝%Z ∗
+        Ψ i
+      else
+        [∗ list] i ∈ seqZ beg (end_ - beg),
+          Χ i
+    }}}.
+  Proof.
+    iIntros "% %Φ (#Hpool_inv & Hctx & Hchunk & Hpred) HΦ".
+
+    wp_rec.
+    wp_smart_apply (algo_adjust_chunk_spec with "[$]"). clear chunk. iIntros "%chunk Hctx".
+
+    iMod (ghost_var_alloc (ghost_var_G := algo_G_find_G) ()) as "(%γ & Htoken)".
+    wp_smart_apply (mvar_create_spec (find_inv γ Ψ beg end_) with "[//]") as (found) "(#Hfound_inv & Hfound_consumer)".
+
+    wp_smart_apply (algo_find_0_spec with "[$]") as "(Hctx & [#Hfound_resolved | (Htoken & HΧ)])"; first done.
+
+    - wp_smart_apply (mvar_try_get_spec_resolved_consumer with "[$]") as (v) "(:find_inv)".
+
+      iSpecialize ("HΦ" $! (Some i)).
+      iSteps.
+
+    - wp_smart_apply (mvar_try_get_spec_consumer with "[$]") as ([v |]) "H".
+
+      + iDestruct "H" as "(_ & (:find_inv =1))".
+        iDestruct (ghost_var_exclusive with "Htoken Htoken_1") as %[].
+
+      + iSpecialize ("HΦ" $! None).
+        iSteps.
+  Qed.
+  Lemma algo_find_spec_nat' (Ψ Χ : nat → iProp Σ) pool sz ctx scope beg end_ chunk pred :
+    (0 ≤ beg ≤ end_)%Z →
+    {{{
+      pool_inv pool sz ∗
+      pool_context pool ctx scope ∗
+      itype_option itype_int chunk ∗
+      [∗ list] (i : nat) ∈ seq ₊beg ₊(end_ - beg),
+        ∀ ctx scope,
+        pool_context pool ctx scope -∗
+        WP pred ctx #i {{ res,
+          ∃ b,
+          ⌜res = #b⌝ ∗
+          pool_context pool ctx scope ∗
+          if b then
+            Ψ i
+          else
+            Χ i
+        }}
+    }}}
+      algo_find ctx #beg #end_ chunk pred
+    {{{ (o : option nat),
+      RET ((#@{nat}) <$> o : option val) : val;
+      pool_context pool ctx scope ∗
+      if o is Some i then
+        ⌜beg ≤ i < end_⌝%Z ∗
+        Ψ i
+      else
+        [∗ list] i ∈ seq ₊beg ₊(end_ - beg),
+          Χ i
+    }}}.
+  Proof.
+    iIntros "% %Φ (#Hpool_inv & Hctx & Hchunk & Hpred) HΦ".
+
+    wp_apply (algo_find_spec'
+      (λ i, Ψ ₊i)
+      (λ i, Χ ₊i)
+    with "[$Hpool_inv $Hctx $Hchunk Hpred]") as (o) "(Hctx & H)"; first lia.
+    { iDestruct (big_sepL_seq_to_seqZ' with "Hpred") as "Hpred"; [lia.. |].
+      iApply (big_sepL_seqZ_impl with "Hpred"). iIntros "!> %k % Hpred".
+      iEval (rewrite Z2Nat.id; try lia) in "Hpred".
+      iSteps.
+    }
+
+    iSpecialize ("HΦ" $! (fmap (FMap := option_fmap) Z.to_nat o)).
+    destruct o as [i |] => /=.
+    - iDestruct "H" as "(% & HΨ)".
+      iEval (rewrite Z2Nat.id; try lia) in "HΦ".
+      iSteps.
+    - iSteps.
+      iApply (big_sepL_seqZ_to_seq' with "H"); lia.
+  Qed.
+  Lemma algo_find_spec (Ψ Χ : Z → iProp Σ) pool sz ctx scope beg end_ chunk pred :
+    (beg ≤ end_)%Z →
+    {{{
+      pool_inv pool sz ∗
+      pool_context pool ctx scope ∗
+      itype_option itype_int chunk ∗
+      □ (
+        ∀ ctx scope i,
+        pool_context pool ctx scope -∗
+        ⌜beg ≤ i < end_⌝%Z -∗
+        WP pred ctx #i {{ res,
+          ∃ b,
+          ⌜res = #b⌝ ∗
+          pool_context pool ctx scope ∗
+          if b then
+            Ψ i
+          else
+            Χ i
+        }}
+      )
+    }}}
+      algo_find ctx #beg #end_ chunk pred
+    {{{ (o : option Z),
+      RET ((#@{Z}) <$> o : option val) : val;
+      pool_context pool ctx scope ∗
+      if o is Some i then
+        ⌜beg ≤ i < end_⌝%Z ∗
+        Ψ i
+      else
+        [∗ list] i ∈ seqZ beg (end_ - beg),
+          Χ i
+    }}}.
+  Proof.
+    iIntros "% %Φ (#Hpool_inv & Hctx & Hchunk & #Hpred) HΦ".
+
+    wp_apply (algo_find_spec' with "[$Hpool_inv $Hctx $Hchunk] HΦ"); first done.
+    { iApply big_sepL_seqZ_intro.
+      iSteps.
+    }
+  Qed.
+  Lemma algo_find_spec_nat (Ψ Χ : nat → iProp Σ) pool sz ctx scope beg end_ chunk pred :
+    (0 ≤ beg ≤ end_)%Z →
+    {{{
+      pool_inv pool sz ∗
+      pool_context pool ctx scope ∗
+      itype_option itype_int chunk ∗
+      □ (
+        ∀ ctx scope (i : nat),
+        pool_context pool ctx scope -∗
+        ⌜beg ≤ i < end_⌝%Z -∗
+        WP pred ctx #i {{ res,
+          ∃ b,
+          ⌜res = #b⌝ ∗
+          pool_context pool ctx scope ∗
+          if b then
+            Ψ i
+          else
+            Χ i
+        }}
+      )
+    }}}
+      algo_find ctx #beg #end_ chunk pred
+    {{{ (o : option nat),
+      RET ((#@{nat}) <$> o : option val) : val;
+      pool_context pool ctx scope ∗
+      if o is Some i then
+        ⌜beg ≤ i < end_⌝%Z ∗
+        Ψ i
+      else
+        [∗ list] i ∈ seq ₊beg ₊(end_ - beg),
+          Χ i
+    }}}.
+  Proof.
+    iIntros "% %Φ (#Hpool_inv & Hctx & Hchunk & #Hpred) HΦ".
+
+    wp_apply (algo_find_spec_nat' with "[$Hpool_inv $Hctx $Hchunk] HΦ"); first done.
     { iApply big_sepL_seq_intro.
       iSteps.
     }
